\chead{Expand Completely}

\newpage
%%%%%%%%%%%%%%%%%%%%%%%%%%%%%%%%%%%%%%%%%%%%%%%%%%%%%%%%%%%%%%%%%%%%%%%%%%%%%%%
%%%
%%%                     EXPAND COMPLETELY
%%%
%%%%%%%%%%%%%%%%%%%%%%%%%%%%%%%%%%%%%%%%%%%%%%%%%%%%%%%%%%%%%%%%%%%%%%%%%%%%%%%
\noindent\subsection*{Expand Completely}
\begin{tcolorbox}[title=Note, colback=blue!10!white, colframe=blue!75!black]
Use the properties to write in simplest form. In particular, use the power, product and quotient rules. 
\end{tcolorbox}
\vspace{0.6cm}
\begin{enumerate}[resume]
    \item $\log_4(x^3)$:
    
    {\color{blue}
        \begin{align*}
        \Aboxed{\log_4(x^3)=3\log_4(x)\makebox[5cm]{\dotfill}\textit{Power Rule}}
    \end{align*}
    }

    
    
    \item $\log_7(49x)$:
    
    {\color{blue}
    \begin{align*}
        \log_7(49x)&=\log_7(49)+\log_7(x)\makebox[5cm]{\dotfill}\textit{Product Rule}\\
        &=\log_7(7^2)+\log_7(x)\\
        \Aboxed{&=2+\log_2(x)\makebox[5cm]{\dotfill}\textit{Inverse Property}}
    \end{align*}
    }


    
    \item $\log_2(5xy)$
    
    {\color{blue}
    \begin{align*}
        \log_2(5xy)&=\log_2(5(xy))\\
        &=\log_2(5)+\log_2(xy)\makebox[7cm]{\dotfill}\textit{Product Rule}\\
        \Aboxed{&=\log_2(5)+\log_2(x)+\log_2(y)\makebox[5cm]{\dotfill}\textit{Product Rule}}
    \end{align*}
    }
    



    \item  $\log_{10}(x^2y^3)$
    
    {\color{blue}
    \begin{align*}
        \log_{10}(x^2y^3)&=\log(x^2+y^2)\makebox[5cm]{\dotfill}\log_{10}u=\log u\\
        &=\log(x^2)+\log(y^3)\makebox[5cm]{\dotfill}\textit{Product Rule}\\
        \Aboxed{&=2\log(x)+3\log(y)\makebox[5cm]{\dotfill}\textit{Power Rule}}
    \end{align*}
    }


    \item  $\log_2\left(\dfrac{x^3y^2}{z^4}\right)$
    
    {\color{blue}
    \begin{align*}
        \log_2\left(\dfrac{x^3y^2}{z^4}\right)&=\log_2(x^3y^2)-\log_2(z^4)\makebox[4cm]{\dotfill}\textit{Quotient Rule}\\
        &=\log_2(x^3)+\log_2(y^2)-\log_2(z^4)\makebox[3cm]{\dotfill}\textit{Product Rule}\\
        \Aboxed{&=3\log_2(x)+2\log_2(y)-4\log_2(z)\makebox[3cm]{\dotfill}\textit{Power Rule}}
    \end{align*}
    }


    \item $\log\left(\dfrac{\sqrt{f^2-3}}{1000}\right)$
    
    {\color{blue}
        \begin{align*}
            \log\left(\dfrac{\sqrt{f^2-3}}{1000}\right)&=\log\left(\dfrac{(f^2-3)^{1/2}}{10^3}\right)\makebox[4cm]{\dotfill}\sqrt{a}=a^{1/2}\\
            &=\log\left(f^2-3\right)^{1/2}-\log\left({10^3}\right)\makebox[2cm]{\dotfill}\textit{Quotient Rule}\\
            &=\dfrac{1}{2}\log\left(f^2-3\right)-3\makebox[2cm]{\dotfill}\textit{Power and Identity Rules}\\
            &=\dfrac{1}{2}\left(\log(f-\sqrt{3})(f+\sqrt{3})\right)-3\makebox[1cm]{\dotfill}a^2-b^2=(a-b)(a+b)\\
            &=\dfrac{1}{2}\left(\log(f-\sqrt{3})+\log(f+\sqrt{3})\right)-3\makebox[1cm]{\dotfill}\textit{Product Rule}\\
            \Aboxed{&=\dfrac{1}{2}\log(f-\sqrt{3}) +\dfrac{1}{2}\log(f+\sqrt{3})-3}\\
        \end{align*}
    }
    


    \item  $\log_3\left(\dfrac{x^2\sqrt[3]{y}}{(z+1)^4}\right)$
    
    {\color{blue}
    \begin{align*}
        \log_3\left(\dfrac{x^2\sqrt[3]{y}}{(z+1)^4}\right)&=\log_3(x^2\sqrt[3]{y})-\log_3(z^4)\makebox[3cm]{\dotfill}\textit{Quotient Rule}\\
        &=\log_3(x^2)+\log_3(y^{1/3})-\log_2((z+1)^4)\makebox[2cm]{\dotfill}\textit{Product Rule}\\
        \Aboxed{&=2\log_3(x)+\dfrac{1}{3}\log_3(y)-4\log_2(z+1)\makebox[2cm]{\dotfill}\textit{Power Rule}}
    \end{align*}
    }

    
    \item  $\log_7\left(\dfrac{\sqrt{x}}{y^2z}\right)$
    
        {\color{blue}
    \begin{align*}
        \log_7\left(\dfrac{\sqrt{x}}{y^2z}\right)&=\log_7(\sqrt{x})-\log_7(y^2z)\makebox[5cm]{\dotfill}\textit{Quotient Rule}\\
        &=\log_7(\sqrt{x})-\left[ \log_7(y^2)+\log_y(z)\right]\makebox[3cm]{\dotfill}\textit{Product Rule}\\
        &=\log_7(x^{1/2})-\log_7(y^2)-\log_y(z)\makebox[3cm]{\dotfill}(\sqrt{x}=x^{1/2})\\
        \Aboxed{&=\dfrac{1}{2}\log_7(x)-2\log_7(y)-\log_7(z)\makebox[3cm]{\dotfill}\textit{Power Rule}}
    \end{align*}
    }
    
    \item  $\log_{e}\left(\dfrac{x^2\sqrt{y}}{z^3}\right)$
    
        {\color{blue}
    \begin{align*}
        \log_{e}\left(\dfrac{x^2\sqrt{y}}{z^3}\right)&=\ln\left(\dfrac{x^2\sqrt{y}}{z^3}\right)\makebox[3cm]{\dotfill}\log_eu=ln u\\
        &=\ln(x^2\sqrt{y})-\ln(z^3)\makebox[3cm]{\dotfill}\textit{Quotient Rule}\\
        &=\ln(x^2)+\ln(\sqrt{y})-\ln(z^3)\makebox[3cm]{\dotfill}\textit{Product Rule}\\
        &=\ln(x^2)+\ln(y^{1/2})-\ln(z^3)\makebox[3cm]{\dotfill}(\sqrt{y}=y^{1/2})\\
        \Aboxed{&=2\ln(x)+\dfrac{1}{2}\ln(y)-3\ln(z)\makebox[3cm]{\dotfill}\textit{Product Rule}}\\
    \end{align*}
    } 



    \item $\log_4\left(\frac{x^3\sqrt[4]{y^3}}{(z^2+1)^{3/2}}\right)$:
    
    {\color{blue}
    \begin{align*}
       \log_4&\left(\frac{x^3\sqrt[4]{y^3}}{(z^2+1)^{3/2}}\right)= \log_4\left(\frac{x^3\,y^{3/4}}{(z^2+1)^{3/2}}\right)\makebox[4cm]{\dotfill}(\sqrt[4]{y^3}=y^{3/4})\\
       &=\log_4\left(x^3\,y^{3/4}\right)-\log_4\left((z^2+1)^{3/2}\right)\makebox[4cm]{\dotfill}\textit{Quotient Rule}\\
       &=\log_4\left(x^3\right)+\log_4\left(y^{3/4}\right)-\log_4\left((z^2+1)^{3/2}\right)\makebox[2cm]{\dotfill}\textit{Product Rule}\\
       \Aboxed{&=3\log_4(x)+\dfrac{3}{4}\log_4(y)-\dfrac{3}{2}\log_4\left(z^2+1\right)\makebox[3cm]{\dotfill}\textit{Power Rule}}\\
    \end{align*}
    }
    

\end{enumerate}