%%%%%%%%%%%%%%%%%%%%%%%%%%%%%%%%%%%%%%%%%%%%%%%%%%%%%%%%%%%%%%%%%%%%%%%%%%%%%%%
%%%
%%%                     New Properties
%%%
%%%%%%%%%%%%%%%%%%%%%%%%%%%%%%%%%%%%%%%%%%%%%%%%%%%%%%%%%%%%%%%%%%%%%%%%%%%%%%%
\newpage
\chead{\textbf{Prove}}

% Optional: add a clearpage if you want the text on its own page
\clearpage 

% Vertical centering: moves the content to the middle of the page
\vspace*{\fill} 

% Horizontal centering: centers the text block horizontally
\begin{center} 
  % Set a very large font size (e.g., 50pt with 60pt line spacing)
  {\fontsize{70}{60}\selectfont 
  \textbf{S O L U T I O N S}
  }
\end{center}

% Vertical centering: balances the 'vspace' above
\vfill 

% Optional: add another clearpage to prevent subsequent text from appearing on the same page
 \clearpage

\newpage

\subsection*{Show That The Statements Are True}


\begin{enumerate}
\item $\log_ac\cdot\log_cb=\log_ab$

    {\color{blue}
\begin{align*}
    \log_ac\cdot\log_cb&=\log_ac\cdot\dfrac{\log_ab}{\log_ac} \makebox[5cm]{\dotfill}\textit{Change of Base}\\
    &=\cancel{\log_ac}\cdot\dfrac{\log_ab}{\cancel{\log_ac}}=\log_ab\qquad\text{QED}
\end{align*}
}

% {\color{blue}
% \begin{align*}
%     \log_ac\cdot\log_cb&=\log_ac\cdot\dfrac{\log_ab}{\log_ac} \makebox[5cm]{\dotfill}\textit{Change of Base}\\
%     &=\cancel{\log_ac}\cdot\dfrac{\log_ab}{\cancel{\log_ac}}=\log_ab\qquad\text{QED}
% \end{align*}
% }
% ---------------------------------------------------------------------------------------

\item $\log_b{1/a}=-\log_b{a}$

{\color{blue}
\begin{align*}
    \log_b{1/a}&=\log_b{1}-\log_b{a}\makebox[5cm]{\dotfill}\textit{Quotient Rule}\\
    &=\cancelto{0}{\log_b{1}}-\log_ba=-\log_ba\makebox[2cm]{\dotfill}\textit{Zero Rule}\quad\text{QED}
\end{align*}
}


% ---------------------------------------------------------------------------------------

\item $\log_ax=-\log_{1/a}x$

{\color{blue}
\begin{align*}
    \log_ax&=y\\
    a^y&=x\makebox[5cm]{\dotfill}\textit{Definition}\\
    \left(\dfrac{1}{a}\right)^{-y}&=x\\
    \log_{1/a}&=-y\makebox[5cm]{\dotfill}\textit{Definition}\\
    y&=-\log_{1/a}x\\
     \log_ax&=-\log_{1/a}x\qquad\text{QED}
\end{align*}
}


% ---------------------------------------------------------------------------------------

\item $\log_{m^n}x^y=\frac{y}{n}\,\log_mx$

    
{\color{blue}
\begin{align*}
    \log_{m^n}x^y&=z\\
    (m^n)^z&=x^y\makebox[5cm]{\dotfill}\textit{Definition}\\
    (m^z)^n&=x^y\\
    m^z&=x^{y/n}\\
    \log_mx^{y/n}&=z\makebox[5cm]{\dotfill}\textit{Definition}\\
    \frac{y}{n}\log_mx&=z\makebox[5cm]{\dotfill}\textit{Power Rule}\\
    \log_{m^n}x^y&=\frac{y}{n}\log_mx\qquad\text{QED}
\end{align*}
}


\end{enumerate}