
\newpage
%%%%%%%%%%%%%%%%%%%%%%%%%%%%%%%%%%%%%%%%%%%%%%%%%%%%%%%%%%%%%%%%%%%%%%%%%%%%%%%
%%%
%%%                     EXPRESS AS A SINGLE LOGARITHM
%%%
%%%%%%%%%%%%%%%%%%%%%%%%%%%%%%%%%%%%%%%%%%%%%%%%%%%%%%%%%%%%%%%%%%%%%%%%%%%%%%%
\subsection*{Express as a single logarithm (when possible)}
\chead{Express As A Single Logarithm}

\begin{tcolorbox}[title=Note, colback=blue!10!white, colframe=blue!75!black]
Use the properties to write in simplest form. In particular, use the power, product and quotient rules but in reverse, for example, for the product rule:  $\log_bM + \log_bN = \log_b(M\cdot N)$. 
\end{tcolorbox}
\vspace{1cm}
\begin{enumerate}[resume]
        \item  $\log_3(5) + \log_3(7)$
        
        {\color{blue}
        \begin{align*}
            \log_3(5) + \log_3(7)&=\log_3(5\times 7)\makebox[5cm]{\dotfill} \textit{Product Property}\\
            \Aboxed{&=\log_3(35)}
        \end{align*}
        }
    

% --------------------------------------------------------------------------------

        \item  $\log_2(12) - \log_2(3)$
        

        {\color{blue}
        \begin{align*}
            \log_2(12) - \log_2(3)&=\log_2\left(\dfrac{12}{3}\right) \makebox[5cm]{\dotfill} \textit{Quotient Property}\\
            &=\log_2(4) &\\
            \Aboxed{&=\log_2{2^2}=2 \makebox[5cm]{\dotfill}\textit{Inverse Property}}
        \end{align*}
        }
        OR
        {\color{teal}
        \begin{align*}
            \log_2(12) - \log_2(3)&=\log_2(4\times 3) - \log_2(3)\\
            &=\log_2{4}+\cancel{\log_2{3}}-\cancel{\log_2{3}} \makebox[2.2cm]{\dotfill}\textit{Product Property}\\
            &=\log_2{4}+\log_2{3}-\log_2{3} &\\
            &=\log_2(4) &\\
            \Aboxed{&=\log_2{2^2}=2 \makebox[5cm]{\dotfill}\textit{Inverse Property}}
        \end{align*}    
        }
    

% --------------------------------------------------------------------------------

        \item $\dfrac{1}{2}\log(z)-\log(z-5)+\log(z^2-25)$
        
        
        {\color{blue}
        \begin{align*}
            \dfrac{1}{2}\log(z)&-\log(z-5)+\log(z^2-25)=\\
            &=\log(z^{1/2})-\log(z-5)+\log\left((z+5)(z-5)\right) \makebox[2cm]{\dotfill} \textit{Power Rule}\\
            &=\log(z^{1/2})-\log(z-5)+\log(z+5) +
            \log(z-5) \makebox[1cm]{\dotfill} \textit{Product Rule}\\
            &=\log(z^{1/2})-\cancel{\log(z-5)}+\log(z+5)+ 
            \cancel{\log(z-5)}\\
            &=\log(z^{1/2})+\log(z+5)\\
            &=\log\left(z^{1/2}(z+5)\right)\makebox[2cm]{\dotfill} \textit{Product Rule}\\
            \Aboxed{&=\log\left(\sqrt{z}\,(z+5)\right)}\\
        \end{align*}
        }
        OR
        {\color{teal}
        \begin{align*}
            \dfrac{1}{2}\log(z)&-\log(z-5)+\log(z^2-25)=\\
            &=\log(z^{1/2})-\log(z-5)+\log\left(z^2-25\right) \makebox[2cm]{\dotfill} \textit{Power Rule}\\
            &=\log\left(\dfrac{z^{1/2}}{z-5}\right)+\log\left(z^2-25\right) \makebox[1cm]{\dotfill} \textit{Quotient Rule}\\
            &=\log\left(\dfrac{z^{1/2}(z^2-25)}{z-5}\right) \makebox[2cm]{\dotfill} \textit{Product Rule}\\
            &=\log\left(\dfrac{z^{1/2}(z+5)(z-5)}{z-5}\right) \makebox[2cm]{\dotfill} a^2-b^2=(a-b)(a+b)\\
            &=\log\left(\dfrac{z^{1/2}(z+5)\cancel{(z-5)}}{\cancel{z-5}}\right) \\\
            &=\log\left(z^{1/2}(z+5)\right)\\
            \Aboxed{&=\log\left(\sqrt{z}\,(z+5)\right)}\\
        \end{align*}
        }
    

% --------------------------------------------------------------------------------


        
        \item $\dfrac{2}{3}\left( 2\ln(x-1)+\ln x-\ln(x^2-9)-3\ln(x+1)\right)$
        
        {\color{blue}
        \begin{align*}
            \dfrac{2}{3}&\left( 2\ln(x-1)+\ln x-\ln(x^2-9)-3\ln(x+1)\right)=\\ &=\dfrac{2}{3}\left(\ln(x-1)^2+\ln x-\ln(x^2-9)-\ln(x+1)^3\right)\makebox[2cm]{\dotfill} \textit{Power Rule}\\
            &=\dfrac{2}{3}\left(\ln x(x-1)^2-\ln(x^2-9)-\ln(x+1)^3\right)\makebox[2cm]{\dotfill} \textit{Product Rule}\\
            % &=\dfrac{2}{3}\left(\ln \left({x(x-1)^2{(x^2-9)}}\right)-\ln(x+1)^3\right)\makebox[2cm]{\dotfill} \textit{Product Rule}\\
            &=\dfrac{2}{3}\left(\ln \left(\dfrac{x(x-1)^2}{x^2-9}\right)-\ln(x+1)^3\right)\makebox[2cm]{\dotfill} \textit{Quotient Rule}\\
            &=\dfrac{2}{3}\ln \left(\dfrac{x(x-1)^2}{(x^2-9)(x+1)^3}\right)\makebox[2cm]{\dotfill} \textit{Quotient Rule}\\
            &=\dfrac{2}{3}\ln \left(\dfrac{x(x-1)^2}{(x-3)(x+3)(x+1)^3}\right)\makebox[2cm]{\dotfill} a^2-b^2=(a-b)(a+b)\\
            \Aboxed{&=\ln \left(\dfrac{x(x-1)^2}{(x-3)(x+3)(x+1)^3}\right)^{2/3}\makebox[2cm]{\dotfill} \textit{Power Rule}}\\
        \end{align*}
        }
    

% --------------------------------------------------------------------------------
        
        
        \item $2\log_5(3)$
        

        {\color{blue}
        \begin{align*}
        \Aboxed{2\log_5(3)=\log_5(3^2)=\log_5(9)\makebox[5cm]{\dotfill} \textit{Power Property}}
        \end{align*}
        }
    

% --------------------------------------------------------------------------------

        \item $\log_6(8) + \log_6(2) - \log_6(4)$
        

        {\color{blue}
        \begin{align*}
           \log_6(8) + \log_6(2) - \log_6(4)&=\log_6(8\times 2) - \log_6(4)\makebox[2cm]{\dotfill}\textit{Product Property}\\
            &=\log_6{16}-\log_6{4} &\\
            &=\log_6\left(\dfrac{16}{4}\right) \makebox[4cm]{\dotfill}\textit{Quotient Property}\\
            \Aboxed{&=\log_6(4)}
        \end{align*}    
        }
        OR (Long way...)
        {\color{teal}
        \begin{align*}
            \log_6(8) &+ \log_6(2) - \log_6(4)=\log_6(4\times 2) +\log_6{2}- \log_6(4)&\\
            &=\cancel{\log_6(4)}+\log_6(2) +\log_6(2)- \cancel{\log_6(4)}\makebox[2cm]{\dotfill}\textit{Product Property}\\
            &=2\log_6{2} &\\
            &=\log_2{2^2} \makebox[8cm]{\dotfill}\textit{Power Property}\\
            \Aboxed{&=\log_6(4)} 
        \end{align*}    
        }
    

% --------------------------------------------------------------------------------


        \item $3\log_4(2) + \log_4(5)$
            

        {\color{blue}
        \begin{align*}
           3\log_4(2) + \log_4(5)&=\log_4(2^3) + \log_4(5)\makebox[3cm]{\dotfill}\textit{Power Property}\\
            &=\log_4(9) + \log_4(5)&\\
            &=\log_4(9\times 5) \makebox[5cm]{\dotfill}\textit{Product Property}\\
            \Aboxed{&=\log_4(45)}
        \end{align*}    
        }
    

% --------------------------------------------------------------------------------


        \item $\frac{1}{2}\log_5(x) - 3\log_5(y) + \log_5(z)$
                

        {\color{blue}
        \begin{align*}
          \frac{1}{2}\log_5(x) - 3\log_5(y) &+ \log_5(z)=&\\
          &=\log_5(x^{\frac{1}{2}}) - \log_5(y^3) + \log_5(z)\makebox[1.2cm]{\dotfill}\textit{Power Property}\\
            &=\log_5(\sqrt{x}) - \log_5(y^3) + \log_5(z)&\\
            &= \log_5\left(\dfrac{\sqrt{x}}{y^3}\right)+ \log_5(z)\makebox[3cm]{\dotfill}\textit{Quotient Property}\\
            \Aboxed{&=\log_5\left(\dfrac{z\,\sqrt{x}}{y^3}\right)\makebox[5cm]{\dotfill}\textit{Product Property}}
        \end{align*}    
        }
    

% --------------------------------------------------------------------------------

        \item $2\log_4(x) + \frac{1}{3}\log_4(y) - 4\log_4(z)$
                

        {\color{blue}
        \begin{align*}
          2\log_4(x) + \frac{1}{3}\log_4(y) &- 4\log_4(z) =&\\
          &=\log_4(x^2) + \log_4(y^{\frac{1}{3}}) - \log_4(z^4)\makebox[2cm]{\dotfill}\textit{Power Property}\\
            &=\log_4(x^2\cdot y^{\frac{1}{3}}) - \log_4(z^4)\makebox[3cm]{\dotfill}\textit{Product Property}\\
            &= \log_4\left(\dfrac{x^2 y^{\frac{1}{3}}}{z^4}\right)\makebox[5cm]{\dotfill}\textit{Quotient Property}\\
            \Aboxed{&=\log_4\left(\dfrac{x^2\sqrt[3]{y}}{z^4}\right)}
        \end{align*}    
        }
    

% --------------------------------------------------------------------------------

        
        \item $\log_6(x) + 2\log_6(y) - \frac{1}{2}\log_6(z)$
                

        {\color{blue}
        \begin{align*}
          \log_6(x) + 2\log_6(y) &- \frac{1}{2}\log_6(z) =&\\
          &=\log_6(x) + \log_6(y^2) - \log_6(z^{\frac{1}{2}})\makebox[2.3cm]{\dotfill}\textit{Power Property}\\
            &=\log_6(x\cdot y^2) - \log_6(z^{\frac{1}{2}})\makebox[4cm]{\dotfill}\textit{Product Property}\\
            &= \log_6\left(\dfrac{x y^2}{z^{\frac{1}{2}}}\right) \makebox[6cm]{\dotfill}\textit{Quotient Property}\\
            \Aboxed{&=\log_6\left(\dfrac{x y^2}{\sqrt{z}}\right)}
        \end{align*}    
        }
      

% --------------------------------------------------------------------------------
      
        
        \item $\log_8(4) + \log_8(16) - \log_8(2)$
                

        {\color{blue}
        \begin{align*}
          \log_8(4) + \log_8(16) &- \log_8(2) = \log_8(4) + \log_8(8\times 2) - \log_8(2)\\
          &=\log_8(4) + \log_8(8)+\cancel{\log_8(2)} - \cancel{\log_8(2)}\makebox[1.3cm]{\dotfill}\textit{Product Property}\\
            &=\log_8(4) + \log_8(8)&\\
            &= \log_8(4\times 8) \makebox[7cm]{\dotfill}\textit{Product Property}\\
            \Aboxed{&=\log_8(32)}
        \end{align*}    
        }
      

% --------------------------------------------------------------------------------
      
    
        \item $\frac{1}{3}\log_6(216) + \frac{2}{5}\log_6(32) - \frac{3}{4}\log_6(81)$
                

        {\color{blue}
        \begin{align*}
          \frac{1}{3}\log_6(216) &+ \frac{2}{5}\log_6(32) - \frac{3}{4}\log_6(81) =&\\
          &=\log_6(216^{1/3}) + \log_6(32^{2/5}) - \log_6(81^{3/4})\makebox[1cm]{\dotfill}\textit{Power Rule}\\
           &=\log_6(6) + \log_6((32^{1/5})^2) - \log_6((81^{1/4})^3)&\\
            &=\log_6(6) + \log_6((2)^2) - \log_6((3)^3)&\\
            &=\log_6(6) + \log_6(4) - \log_6(27)&\\
            &=\log_6(6\times 4) - \log_6(27)\makebox[5cm]{\dotfill}\textit{Product Rule}\\
            \Aboxed{&= \log_6\left(\dfrac{24}{27}\right) \makebox[7cm]{\dotfill}\textit{Quotient Rule}}\\
        \end{align*}    
        }
     

% --------------------------------------------------------------------------------
   
    \item $ \sum_{k=1}^{n} \log_a(k)$
            

    {\color{blue}
    \begin{align*}
      \sum_{k=1}^{n} \log_a(k)&=\log_a(1) +\log_a(2)+\cdots +\log_a(n-1)+\log_a(n)&\\
       &=\log_a(n) +\log_a(n-1)+\cdots +\log_a(2)+\log_a(1)\makebox[1cm]{\dotfill}\textit{reverse the sum}\\
        &=\log_a(n\cdot (n-1)\cdots 2\cdot 1)\makebox[5cm]{\dotfill}\textit{Product Rule}\\
        \Aboxed{&=\log_a(n!)}
    \end{align*}    
    }
    

% --------------------------------------------------------------------------------

\end{enumerate}