

\section*{Rewrite using positive exponents}
\begin{enumerate}
    
\item $t^{-5}$\\

{\color{blue}
Solution:
\begin{align*}
   t^{-5} &=
\end{align*}
}


\item $5^{-3}$\\

{\color{blue}
Solution:
\begin{align*}
    5^{-3}&=
\end{align*}
}


\item $8^{-2}$\\

{\color{blue}
Solution:
\begin{align*}
  8^{-2}  &=
\end{align*}
}


\item $4^{-6}$\\

{\color{blue}
Solution:
\begin{align*}
   4^{-6} &=
\end{align*}
}


\item $10^{-3}$\\

{\color{blue}
Solution:
\begin{align*}
  10^{-3}  &=
\end{align*}
}


\item $-7w^{-3}$\\

{\color{blue}
Solution:
\begin{align*}
    -7w^{-3}&=
\end{align*}
}


\item $(-7w)^{-3}$\\

{\color{blue}
Solution:
\begin{align*}
   (-7w)^{-3} &=
\end{align*}
}


\item $18q^{-2}$\\

{\color{blue}
Solution:
\begin{align*}
   18q^{-2} &=
\end{align*}
}


\item $-5c^{-4}$\\

{\color{blue}
Solution:
\begin{align*}
   -5c^{-4} &=
\end{align*}
}


\item $(-5c)^{-4}$\\

{\color{blue} 
Solution:
\begin{align*}
    (-5c)^{-4}&=\dfrac{1}{(-5c)^4}\qquad\qquad \text{negative exponent}\\
    &=\dfrac{1}{(-5)^4c^4}\qquad\qquad\text{product to a power}\\
    &=\dfrac{1}{625c^4}
\end{align*}

}

\item  $\dfrac{9p^3}{4q^{-4}}$\\

{\color{blue}
Solution:
\begin{align*}
    \dfrac{9p^3}{4q^{-4}}&=\dfrac{9p^3q^4}{4}\qquad\qquad\text{negative exponent}
\end{align*}


}

\item $\dfrac{24r^{-4}}{12s^{-5}}$\\

{\color{blue}
Solution:
\begin{align*}
    \dfrac{24r^{-4}}{12s^{-5}}&=\dfrac{\cancelto{2}{24}s^5}{\cancel{12}r^4}\qquad\qquad\text{negative exponent}\\
    &=\dfrac{2s^5}{r^4}
\end{align*}


}

\item $\dfrac{1}{5t^{-5}}$\\

{\color{blue}
Solution:
\begin{align*}
    \dfrac{1}{5t^{-5}}&=\dfrac{t^5}{5}\qquad\qquad\text{Negative exponent}
\end{align*}
}

\item $\dfrac{1}{6w^{-2}}$\\

{\color{blue}
Solution:
\begin{align*}
   \dfrac{1}{6w^{-2}} &=
\end{align*}
}

\item $\dfrac{d^{-4}}{5}$\\

{\color{blue}
Solution:
\begin{align*}
   \dfrac{d^{-4}}{5} &=
\end{align*}
}


\item $\dfrac{e^{-5}}{9}$\\

{\color{blue}
Solution:
\begin{align*}
   \dfrac{e^{-5}}{9} &=
\end{align*}
}


\item $\dfrac{5^{-3}}{z}$\\

{\color{blue}
Solution:
\begin{align*}
   \dfrac{5^{-3}}{z} &=
\end{align*}
}


\item $\dfrac{7^{-2}}{y^3}$\\

{\color{blue}
Solution:
\begin{align*}
    \dfrac{7^{-2}}{y^3}&=
\end{align*}
}

\end{enumerate}

\section{Simplify and write using positive exponents only}
\begin{enumerate}[resume]

\item $\dfrac{z^4}{z^9}$\\

{\color{blue}
Solution:
\begin{align*}
   \dfrac{z^4}{z^9} &=
\end{align*}
}


\item $\dfrac{c^5}{c^{12}}$\\

{\color{blue}
Solution:
\begin{align*}
    \dfrac{c^5}{c^{12}}&=
\end{align*}
}


\item $\dfrac{m^3n^2}{m^6n^4}$\\

{\color{blue}
Solution:
\begin{align*}
    \dfrac{m^3n^2}{m^6n^4}&=
\end{align*}
}


\item $\dfrac{t^4u^3}{tu^7}$\\

{\color{blue}
Solution:
\begin{align*}
    \dfrac{t^4u^3}{tu^7}&=
\end{align*}
}


\item $\dfrac{15p^7q^9}{10p^{13}q^3}$\\

{\color{blue}
Solution:
\begin{align*}
    \dfrac{15p^7q^9}{10p^{13}q^3}&=
\end{align*}
}


\item $\dfrac{18r^3s^6}{24r^8s^3}$\\

{\color{blue}
Solution:
\begin{align*}
    \dfrac{18r^3s^6}{24r^8s^3}&=
\end{align*}
}


\item $\dfrac{8w^4v^{-3}}{w^7v^5}$\\

{\color{blue}
Solution:
\begin{align*}
   \dfrac{8w^4v^{-3}}{w^7v^5} &=
\end{align*}
}


\item $\dfrac{12x^5y^{-2}}{xy^4}$\\

{\color{blue}
Solution:
\begin{align*}
   \dfrac{12x^5y^{-2}}{xy^4} &=
\end{align*}
}


\item $\dfrac{20h^{-2}k^6}{15h^3k^{-2}}$\\

{\color{blue}
Solution:
\begin{align*}
   \dfrac{20h^{-2}k^6}{15h^3k^{-2}} &=
\end{align*}
}


2\item $\dfrac{42g^{-5}f^3}{18g^4f^{-3}}$\\

{\color{blue}
Solution:
\begin{align*}
    \dfrac{42g^{-5}f^3}{18g^4f^{-3}}&=
\end{align*}
}


\item $\dfrac{-30m^3n^{-5}}{10mn^2}$\\

{\color{blue}
Solution:
\begin{align*}
    \dfrac{-30m^3n^{-5}}{10mn^2}&=
\end{align*}
}


\item $\dfrac{-54p^5q^{-4}}{18pq^3}$\\

{\color{blue}
Solution:
\begin{align*}
    \dfrac{-54p^5q^{-4}}{18pq^3}&=
\end{align*}
}


\item $\left(4r^{-3}\right)^3$\\

{\color{blue}
Solution:
\begin{align*}
    \left(4r^{-3}\right)^3&=
\end{align*}
}


\item $\left(5s^{-2}\right)^4$\\

{\color{blue}
Solution:
\begin{align*}
    \left(5s^{-2}\right)^4&=
\end{align*}
}


\item $\left(-7t^{-4}\right)^2$\\

{\color{blue}
Solution:
\begin{align*}
   \left(-7t^{-4}\right)^2 &=
\end{align*}
}


\item $\left(-5u^{-5}\right)^2$\\

{\color{blue}
Solution:
\begin{align*}
    \left(-5u^{-5}\right)^2&=
\end{align*}
}


\item $\left(-5v^{-3}\right)^2\left(-10v^4w^{-2}\right)$\\

{\color{blue}
Solution:
\begin{align*}
   \left(-5v^{-3}\right)^2\left(-10v^4w^{-2}\right) &=
\end{align*}
}


\item $\left(-4a^{-2}\right)^4\left(-8ab^{-2}\right)$\\

{\color{blue}
Solution:
\begin{align*}
    \left(-4a^{-2}\right)^4\left(-8ab^{-2}\right)&=
\end{align*}
}


\item $\left(\dfrac{-6c^6d^4}{9c^9d^{-2}}\right)^2$\\

{\color{blue}
Solution:
\begin{align*}
    \left(\dfrac{-6c^6d^4}{9c^9d^{-2}}\right)^2&=
\end{align*}
}


\item $\left(\dfrac{-21m^4n^3}{49m^{-3}n^5}\right)^2$\\

{\color{blue}
Solution:
\begin{align*}
    \left(\dfrac{-21m^4n^3}{49m^{-3}n^5}\right)^2&=
\end{align*}
}


\item $\left(\dfrac{q}{p^2}\right)^{-3}$\\

{\color{blue}
Solution:
\begin{align*}
    \left(\dfrac{q}{p^2}\right)^{-3}&=
\end{align*}
}


\item $\left(\dfrac{r^3}{s^2}\right)^{-4}$\\

{\color{blue}
Solution:
\begin{align*}
    \left(\dfrac{r^3}{s^2}\right)^{-4}&=
\end{align*}
}

\end{enumerate}


\section{Simplify each expression}

\begin{enumerate}[resume]
\item $(-5)^2$\\

{\color{blue}
Solution:
\begin{align*}
    (-5)^2&=
\end{align*}
}


\item $-5^2$\\

{\color{blue}
Solution:
\begin{align*}
    -5^2
\end{align*}
}


\item  $(-5)^3$\\

{\color{blue}
Solution:
\begin{align*}
    (-5)^3
\end{align*}
}


\item  $-5^3$\\

{\color{blue}
Solution:
\begin{align*}
    -5^3&=
\end{align*}
}


\item $(-7)^2$\\

{\color{blue}
Solution:
\begin{align*}
    (-7)^2&=
\end{align*}
}


\item $c^5d^4$\\

{\color{blue}
Solution:
\begin{align*}
    c^5d^4&=
\end{align*}
}


\item $4^5 \cdot 4^2$\\

{\color{blue}
Solution:
\begin{align*}
    4^5 \cdot 4^2&=
\end{align*}
}


\item $5t^5 \cdot 6t^9$\\

{\color{blue}
Solution:
\begin{align*}
    5t^5 \cdot 6t^9&=5\times 6\cdot t^5\times t^6\\
    &=30\,t^{5+6}\\
    &=30\,t^{11}
\end{align*}
}


\item $8u^4 \cdot 9u \cdot 4u^5$\\

{\color{blue}
Solution:
\begin{align*}
    8u^4 \cdot 9u \cdot 4u^5&=8\times 9\times 4\cdot u^4\times u\times u^5\\
    &=288\cdot u^{4+1+5}\\
    &=288\,u^{10}
\end{align*}
}


\item $9vw^3\left(11v^6w^4\right)$\\

{\color{blue}
Solution:
\begin{align*}
    9vw^3\left(11v^6w^4\right)&=9\times 11\cdot v\times v^6\cdot w^3\times w^4\\
    &=99\,v^{1+6}\,w^{3+4}
\end{align*}
}


\item $10x^6y^5\left(4xy^3\right)$\\

{\color{blue}
Solution:
\begin{align*}
    10x^6y^5\left(4xy^3\right)
\end{align*}
}


\item $-6p^4q^5\left(7p^8q^4\right)$\\

{\color{blue}
Solution:
\begin{align*}
    -6p^4q^5\left(7p^8q^4\right)&=-6\times 7\cdot p^4\times p^8\cdot q^5\times q^4\\
    &=-42\,p^{4+8}\,q^{5+4}\\
    &=-42\,p^{12}\,q^{9}
\end{align*}
}


\item $-4r\left(5r^3s^4\right)^{2}\left(-6rs^2\right)^{-2}\left(-s^{-6}\right)$\\

{\color{blue}
Solution:
\begin{align*}
    -4r\left(5r^3s^4\right)^{2}\left(-6rs^2\right)^{-2}\left(-s^{-6}\right)&=
    \dfrac{-4r(5r^3s^4)^2}{-s^6(-6rs^2)^2}\\
    &=\dfrac{4r\cdot 5^2\,r^{3\times 2}s^{4\times 2}}{s^6\cdot (-6)^2r^2s^{2\times 2}}\\
    &=\dfrac{20r.r^6s^8}{36s^6r^2s^6}=\dfrac{\cancelto{5}{20}r^{1+6}s^8}{\cancelto{9}{36}r^2s^{6+4}}\\
    &=\dfrac{5r^7s^8}{9r^2s^{10}}=\dfrac{5r^{7-2}}{9s^{10-8}}\\
    &=\dfrac{5r^5}{9w^2}
\end{align*}
}


\item $(2a^3)^6\cdot(3a)^4$\\

{\color{blue}
Solution:
\begin{align*}
    (2a^3)^6\cdot(3a)^4&=2^6a^{3\times 6}\cdot 3^4 a^4\\
    &=64\times 81\cdot a^{18}\times a^4\\
    &=5184a^{18+4}=5184a^{22}
\end{align*}
}


\item $(2c)^3 \cdot (2c)^5$\\

{\color{blue}
Solution:
\begin{align*}
    (2c)^3 \cdot (2c)^5&=2^3\,c^3\cdot 2^5c^5\\
    &=2^{2+5}c^{3+5}\\
    &=2^8c^8=256c^8
\end{align*}
}


\item $(-2n)^\cdot(-2n)^3$\\

{\color{blue}
Solution:
\begin{align*}
    (-2n)^4\cdot(-2n)^3&=(-2)^4n^4\cdot(-2)^3n^3\\
    &=-2^4\times 2^3\cdot n^4\times n^3\\
    &=-2^{4+3}\,n^{6+4}\\
    &=-2^7\,n^7=-128\,n^7
\end{align*}
}


\item  $\dfrac{t^{14}}{t^6}$\\

{\color{blue}
Solution:
\begin{align*}
    \dfrac{t^{14}}{t^6}&=t^{14-6}=t^8
\end{align*}
}


\item  $\dfrac{30m^{19}}{6m^4}$\\

{\color{blue}
Solution:
\begin{align*}
    \dfrac{30m^{19}}{6m^4}&=5m^{19-4}=5m^{15}
\end{align*}
}


\item $\dfrac{g^{18}}{g^{13}}$\\

{\color{blue}
Solution:
\begin{align*}
   \dfrac{g^{18}}{g^{13}} &=g^{18-13}=g^5
\end{align*}
}


\item $\dfrac{63p^8}{7p}$\\

{\color{blue}
Solution:
\begin{align*}
  \dfrac{63p^8}{7p}  &=9p^{8-1}=9p^7
\end{align*}
}


\item  $\left(\dfrac{-5r^8s^6}{r^3s^4}\right)^{-4}$\\

{\color{blue}
Solution:
\begin{align*}
    \left(\dfrac{-5r^8s^6}{r^3s^4}\right)^{-4}&=\left(\dfrac{r^3s^4}{-5r^8s^6}\right)^4\\
    &=\left(\dfrac{1}{-5r^{8-4}s^{6-4}}\right)^4\\
    &=\left(\dfrac{1}{-5r^4s^2}\right)^4\\
    &=\dfrac{1}{(-5)^4r^{4\times 4}s^{2\times 4}}\\
    &=\dfrac{1}{625r^{16}s^8}
\end{align*}
}


\item $\left(\dfrac{8u^4}{4}\right)^2(4u^3v^5)^3$\\

{\color{blue}
Solution:
\begin{align*}
    \left(\dfrac{8u^4}{4}\right)^2(4u^3v^5)^3&=\left(2u^4\right)^2(2^2u^3v^5)^3\\
    &=2^2u^{4\times 2}\cdot2^{2\times 3}u^{3\times 3}v^{5\times 3}\\
    &=2^2u^8\cdot 2^6u^9v^{15}\\
    &=2^{2+6}u^{8+9}v^{15}\\
    &=2^8u^{17}v^{15}=256u^{17}v^{15}
\end{align*}
}


\item $-4w^6z^4\left(8w^4z^6\right)^2$\\

{\color{blue}
Solution:
\begin{align*}
    -4w^6z^4\left(8w^4z^6\right)^2
\end{align*}
}


% \item $(7h)^6(7h)^9$\\

% {\color{blue}
% Solution:
% \begin{align*}
%     (7h)^6(7h)^9
% \end{align*}
% }


\item  $\left(k^3\right)^6$\\

{\color{blue}
Solution:
\begin{align*}
    \left(k^3\right)^6&=k^{3\times 6}=k^{18}
\end{align*}
}


\item  $\left(f^5\right)^4$\\

{\color{blue}
Solution:
\begin{align*}
    \left(f^5\right)^4&=f^{5\times 4}=f^{20}
\end{align*}
}


\item $\left(b^3c^7\right)^6$\\

{\color{blue}
Solution:
\begin{align*}
    \left(b^3c^7\right)^6&=\left(b^3\right)^6\left(c^7\right)^6\\
    &=b^{3\times 6}\,c^{7\times 6}\\
    &=b^{18}\,c^{42}
\end{align*}
}


\item  $\left(d^7f^{-6}\right)^5$\\

{\color{blue}
Solution:
\begin{align*}
    \left(d^7f^{-6}\right)^5&=\left(d^7\right)^5\left(f^{-6}\right)^5\\
    &=d^{7\times 5}f^{-6\times 5}\\
    &=d^{35}f^{-30}\\
    &=\dfrac{d^{35}}{f^{30}}
\end{align*}
}

\end{enumerate}

\section{Simplify using exponent rules}

\begin{enumerate}[resume]

\item $\dfrac{p^3p^6q^7}{p^5q^3}$\\

{\color{blue}
Solution:
\begin{align*}
    \dfrac{p^3p^6q^7}{p^5q^3}&=\dfrac{p^{3+6q^7}}{p^5q^3}\\
    &=\dfrac{p^9q^7}{p^5q^3}\\
    &=p^{9-5}q^{7-3}\\
    &=p^4q^4
\end{align*}
}


\item $\dfrac{r^7r^3s^6}{r^5r^4s}$\\

{\color{blue}
Solution:
\begin{align*}
    \dfrac{r^7r^3s^6}{r^5r^4s}&=\dfrac{r^{7+3}s^6}{r^{5+4}s}\\
    &=\dfrac{r^{10}s^6}{r^{9}s}\\
    &=r^{10-9}s^{6-1}\\
    &=rs^5
\end{align*}
}


\item $\dfrac{t^3t^4u^3}{tu}$\\

{\color{blue}
Solution:
\begin{align*}
    \dfrac{t^3t^4u^3}{tu}&=\dfrac{t^{3+4}u^3}{tu}\\
    &=\dfrac{t^7u^3}{tu}\\
    &=t^{7-1}u^{3-1}\\
    &=t^6u^2
\end{align*}
}


\item $\dfrac{v^5v^8w^4w^3}{v^4vw^5}$\\

{\color{blue}
Solution:
\begin{align*}
    \dfrac{v^5v^8w^4w^3}{v^4vw^5}&=\dfrac{v^{5+8}w^{4+3}}{v^{4+1}w^5}\\
    &=\dfrac{v^{13}w^{7}}{v^{5}w^5}\\
    &=v^{13-5}w^{7-5}\\
    &=v^8 w^2
\end{align*}
}


\item $\dfrac{9x^6y^4}{18x^6y^7}$\\

{\color{blue}
Solution:
\begin{align*}
   \dfrac{9x^6y^4}{18x^6y^7} &=\dfrac{\cancel{x^6}}{2\cancel{x^6}y^{7-4}}\\
   &=\dfrac{1}{2y^3}
\end{align*}
}


\item  $\dfrac{-6z^3a^3}{24z^8a}$\\

{\color{blue}
Solution:
\begin{align*}
    \dfrac{-6z^3a^3}{24z^8a}&=\dfrac{-a^{3-1}}{4z^{8-3}}\\
    &=-\dfrac{a^2}{4z^5}
\end{align*}
}


\item $\dfrac{48b^6c^3}{20bc^3}$\\

{\color{blue}
Solution:
\begin{align*}
   \dfrac{48b^6c^3}{20bc^3} &=\dfrac{\cancelto{12}{48}b^{6-1}\cancel{c^3}}{\cancelto{5}{20}\cancel{c^3}}\\
   &=\dfrac{12b^5}{5}
\end{align*}
}


\item $\dfrac{-25de^{-6}}{10d^4e}$\\

{\color{blue}
Solution:
\begin{align*}
    \dfrac{-25de^{-6}}{10d^4e}&=\dfrac{-\cancelto{5}{25}}{\cancelto{2}{10}d^{4-1}e^{1+6}}\\
    &=-\dfrac{5}{2d^3e^7}
\end{align*}
}


\item $\dfrac{f^5}{42} \cdot \dfrac{7}{f^3}$\\

{\color{blue}
Solution:
\begin{align*}
    \dfrac{f^5}{42} \cdot \dfrac{7}{f^3}&=\dfrac{f^{5-3}}{6}\\
    &=\dfrac{f^2}{6}
\end{align*}
}


\item $\dfrac{-18}{g} \cdot \frac{g^6}{6}$\\

{\color{blue}
Solution:
\begin{align*}
    \dfrac{-18}{g} \cdot \frac{g^6}{6}&=
\end{align*}
}


\item $\dfrac{h^5k}{h^3k} \cdot \frac{k^4}{h}$\\

{\color{blue}
Solution:
\begin{align*}
    \dfrac{h^5k}{h^3k} \cdot \frac{k^4}{h}&=
\end{align*}
}


\item  $\dfrac{mn^6}{mn^3} \cdot \frac{m^5n^4}{mn}$\\

{\color{blue}
Solution:
\begin{align*}
    \dfrac{mn^6}{mn^3} \cdot \frac{m^5n^4}{mn}&=
\end{align*}
}


\item  $\dfrac{24p^3q^7}{pq^4} \cdot \frac{p^4q^3}{72pq^3}$\\

{\color{blue}
Solution:
\begin{align*}
    \dfrac{24p^3q^7}{pq^4} \cdot \frac{p^4q^3}{72pq^3}&=
\end{align*}
}


\item  $\dfrac{-15r^4s^8}{r^3s^3} \cdot \frac{rs^4}{36rs^3}$\\

{\color{blue}
Solution:
\begin{align*}
    \dfrac{-15r^4s^8}{r^3s^3} \cdot \frac{rs^4}{36rs^3}&=
\end{align*}
}


\item  $\left(5t^3u^6\right)^2$\\

{\color{blue}
Solution:
\begin{align*}
    \left(5t^3u^6\right)^2&=
\end{align*}
}


\item $\left(5vw^5\right)^3$\\

{\color{blue}
Solution:
\begin{align*}
   \left(5vw^5\right)^3 &=5^3v^3w^{5\times 3}\qquad\text{{\scriptsize product and power to a power}} \\
   &=125\,v^3\,w^15
\end{align*}
}


\item $\left(-7x^8y^{-6}\right)^2$\\

{\color{blue}
Solution:
\begin{align*}
    \left(-7x^8y^{-6}\right)^2&=(-7)^2x^{8\times 2}y^{-6\times 2}\qquad\text{{\scriptsize product and power to a power}} \\
    &=49\,x^{16}\,y^{-12}\\
    &=\dfrac{49x^{16}}{y^{12}}\qquad\text{{\scriptsize negative exponent rule}} \\
\end{align*}
}


\item $\left(-4z^3a^9\right)^4$\\

{\color{blue}
Solution:
\begin{align*}
    \left(-4z^3a^9\right)^4&=
\end{align*}
}


\item $\left(20b^{12}c^6\right)^0$\\

{\color{blue}
Solution:
\begin{align*}
  \left(20b^{12}c^6\right)^0  &=
\end{align*}
}


\item $\left(-10d^9e^5\right)^0$\\

{\color{blue}
Solution:
\begin{align*}
   \left(-10d^9e^5\right)^0 &=
\end{align*}
}


\item  $\left(\dfrac{18f^6g^5}{3f^3g}\right)^2$\\

{\color{blue}
Solution:
\begin{align*}
    \left(\dfrac{18f^6g^5}{3f^3g}\right)^2&=
\end{align*}
}


\item $\left(\dfrac{32h^8k^6}{8h^4k^3}\right)^3$\\

{\color{blue}
Solution:
\begin{align*}
   \left(\dfrac{32h^8k^6}{8h^4k^3}\right)^3 &=\left(\dfrac{\cancelto{4}{32}h^8k^6}{\cancel{8}h^4k^3}\right)^3\\
   &=\left(4h^{8-4}k^{6-3}\right)^3\qquad\qquad\text{quotient rule}\\
   &=\left(4h^{4}k^{3}\right)^3\\
   &=4^4h^{4\times 3}k^{3\times 3}\qquad\text{product to a power and power to a power}\\
   &=64\,h^{12}\,k^9
\end{align*}
}


\item $\left(\dfrac{-36m^4n^6}{9mn}\right)^2$\\

{\color{blue}
Solution:
\begin{align*}
   \left(\dfrac{-36m^4n^6}{9mn}\right)^2 &=
\end{align*}
}


\item  $\left(\dfrac{-30p^9q^3}{6p^6q}\right)^2$\\

{\color{blue}
Solution:
\begin{align*}
    \left(\dfrac{-30p^9q^3}{6p^6q}\right)^2&=
\end{align*}
}


\item  $\left(\dfrac{15r^{-4}}{5s^6}\right)^0$\\

{\color{blue}
Solution:
\begin{align*}
    \left(\dfrac{15r^{-4}}{5s^6}\right)^0&=
\end{align*}
}


\item $\left(\dfrac{24t^{-6}}{-6u^{-3}}\right)^0$\\

{\color{blue}
Solution:
\begin{align*}
    \left(\dfrac{24t^{-6}}{-6u^{-3}}\right)^0&=1\qquad\qquad\text{{\scriptsize zero power rule}}
\end{align*}

Here we assume that the quantity in parenthesis $\left(\dfrac{24t^{-6}}{-6u^{-3}}\right)$ is not zero. Otherwise, if that quantity is zero, then the expression is undefined. 
}

\item $5vw^3\left(7v^4w^8\right)^{-2}$\\

{\color{blue}
Solution:
\begin{align*}
   5vw^3\left(7v^4w^8\right)^{-2} &=\dfrac{5vw^3}{\left(7v^4w^8\right)^2}\qquad\text{{\scriptsize negative exponent rule}}\\
   &=\dfrac{5vw^3}{7^2v^{4\times 2}w^{8\times 2}}\qquad\text{{\scriptsize product and power to a power rule}}\\
   &=\dfrac{5vw^3}{7^2v^8w^{16}}\\
   &=\dfrac{5}{49\,v^{8-1}\,w^{16-3}}\qquad\text{{\scriptsize quotient and negative exponent rule}}\\
   &=\dfrac{5}{49\,v^{7}\,w^{13}}
\end{align*}
}


\item  $4x^6y^{-4}\left(8x^{-3}y^3\right)^{-2}$\\

{\color{blue}
Solution:
\begin{align*}
    4x^6y^{-4}\left(8x^{-3}y^3\right)^{-2}&=\dfrac{4x^6}{y^4\left(8x^{-3}y^3\right)^2}\qquad\text{{\scriptsize negative power rule}}\\
    &=\dfrac{4x^6}{y^4\cdot 8^2x^{-3\times 2}y^{3\times 2}}\qquad\text{{\scriptsize product and power to a power rule}} \\
    &=\dfrac{4x^6}{y^4\cdot 64, x^{-6}y^6}\\
    &=\dfrac{x^{6+6}}{16y^{4+6}}\qquad\text{{\scriptsize product and quotient rule}} \\
    &=\dfrac{x^{12}}{16y^{10}}
\end{align*}
}


\item $6z^5a^4\left(5za^6\right)^3$\\

{\color{blue}
Solution:
\begin{align*}
   6z^5a^4\left(5za^6\right)^3 &=
\end{align*}
}


\item $9b^8c^3\left(4b^5c^7\right)^2$\\

{\color{blue}
Solution:
\begin{align*}
    9b^8c^3\left(4b^5c^7\right)^2&=9b^8c^3\cdot 4^2b^{5\times 2}c^{7\times 2}\qquad\qquad\text{{\scriptsize product to a power}}\\
    &=9b^8c^3\cdot 16b^{10}c^{14}\\
    &=9\times 16 \cdot b^8\times b^{10}\cdot c^3\times c^{14}\\
    &=144\,b^{8+10}c^{3+14}\qquad\qquad\text{{\scriptsize product rule}}\\
    &=144\,b^{18}c^{17}
\end{align*}
}


\item  $-5d^3\left(4dg^4\right)^3$\\

{\color{blue}
Solution:
\begin{align*}
   -5d^3\left(4dg^4\right)^3 &=-5d^3\cdot 4^3d^3g^{4\times 3}\qquad \text{{\scriptsize product and power to a power rule}}\\
   &=-5\times 64\cdot d^3\times d^3\cdot g^{12}\\
   &=-320\,d^{3+3}\,g^{12}\\
   &=-320\,d^6\,g^{12}
\end{align*}
}


\item  $-7f^2\left(6f^4g\right)^2$\\

{\color{blue}
Solution:
\begin{align*}
    -7f^2\left(6f^4g\right)^2&=
\end{align*}
}


\item  $(4h^4k)^5(7hk^3)^2$\\

{\color{blue}
Solution:
\begin{align*}
   (4h^4k)^5(7hk^3)^2 &=
\end{align*}
}


\item  $(8m^4n^6)^2(5mn^3)^3$\\

{\color{blue}
Solution:
\begin{align*}
    (8m^4n^6)^2(5mn^3)^3&=
\end{align*}
}


\item  $(-3p^6q^4)^2(-2p^3q)^3$\\

{\color{blue}
Solution:
\begin{align*}
    (-3p^6q^4)^2(-2p^3q)^3&=(-3)^2p^{6\times 2}q^{4\times 2}\cdot (-2)^3p^{3\times 3}q^3\qquad\text{{\scriptsize product and power to a power rule}}\\
    &=9\,p^{12} q^8\cdot (-8)\,p^9q^3\\
    &=9\times (-8)\cdot p^{12}\times p^9\cdot q^8\times q^3\\
    &=-72\,p^{12+9}\,q^{8+3}\qquad\qquad\text{{\scriptsize product rule}}\\
    &=-72\,p^{21}\,q^{11}
\end{align*}
}


\item  $(-4r^5s^4)^4(4r^4s^3)^{-3}$\\

{\color{blue}
Solution:
\begin{align*}
    (-4r^5s^4)^4(4r^4s^3)^{-3}&=\dfrac{(-4r^5s^4)^4}{(4r^4s^3)^3}\qquad\text{{\scriptsize negative exponent rule}}\\
    &=\dfrac{(-4)^4r^{5\times 4}s^{4\times 4}}{4^3r^{4\times 3}s^{3\times 3}}\qquad\text{{\scriptsize product and power to a power}}\\
    &=\dfrac{4^4r^{20}s^{16}}{4^3r^{12}s^9}\\
    &=4^{4-3}\,r^{20-12}\,s^{16-9}\qquad\text{{\scriptsize quotient rule}}\\
    &=4\,r^8\,s^7
\end{align*}
}

\end{enumerate}
